---
title: "Trigonometric Identities (problem solving)"
date: 04-12-2022
weight: 4
url: /Trigonometric-Identities-(problem-solving)/
mathjax: true
---


### If cos 2A = $tan^2$ B then find the value of  $tan^2$ A in terms of B.

**Sol:**

Given, cos 2A = $tan^2$ B

Use multiple angle formula of cos, i.e. cos 2A = $\frac{1- tan^2\ A}{1+ tan^2\ A}$

$\frac{1- tan^2\ A}{1+ tan^2\ A}$ = $tan^2$ B

1- $tan^2$ A = $tan^2$ B (1+ $tan^2$ A)

1- $tan^2$ A = $tan^2$ B + $tan^2$ B $tan^2$ A

1- $tan^2$ B = $tan^2$ A + $tan^2$ B $tan^2$ A

1- $tan^2$ B = $tan^2$ A(1- $tan^2$ B)

$\frac{1- tan^2\ B}{1+ tan^2\ B}$ = $tan^2$ A

Again use the formula cos 2A = $\frac{1- tan^2\ A}{1+ tan^2\ A}$

cos 2B = $tan^2$ A

Therefore $tan^2$ A = cos 2B

### If a cos A - b sin A = c then find the value of a sin A + b cos A

**Sol:**

Given, a cos A - b sin A = c

Squaring on both sides

$(a cos A - b sin A)^2$ = $c^2$

$a^2\ cos^2$ A + $b^2\ sin^2$ A -2ab sin A cos A = $c^2$

$a^2\ (1-sin^2$ A) + $b^2\ (1-sin^2$ A) -2ab sin A cos A = $c^2$

$a^2$ - $a^2\ sin^2$ A + $b^2$ - $b^2\ sin^2$ A -2ab sin A cos A = $c^2$

$a^2$ + $b^2$ - ( $a^2\ sin^2$ A + $b^2\ sin^2$ A + 2ab sin A cos A) = $c^2$

(a sin A + b cos A $)^2$ = $a^2$ + $b^2$ - $c^2$

a sin A + b cos A = $\pm \sqrt{a^2 + b^2 - c^2}$

### If sin A + cosec A = 2 then find the value of sin $^20$ A + cosec $^20$ A

**Sol:**

sin A + cosec A = 2

sin A + $\frac{1}{sin\ A}$ = 2

Sin $^2$ A + 1 = 2 sin A

Sin $^2$ A + 1 - 2 sin A = 0

(sin A - 1 $)^2$ = 0

Sin A = 1

So cosec A = 1

sin $^20$ A + cosec $^20$ A =1+1

sin $^20$ A + cosec $^20$ A = 2

### If sin A + sin $^2$ A + sin $^3$ A = 1 find the value of cos $^6$ A - 4cos $^4$ A + 8cos $^2$

**Sol:**

Given, sin A + sin $^2$ A + sin $^3$ A = 1

sin A + sin $^3$ A = 1- sin $^2$ A

sin A + sin $^3$ A = cos $^2$ A

Square on both sides

( sin A + sin $^3$ A $)^2$ = cos $^4$ A

sin $^2$ A + 2sin $^4$ A + sin $^6$ A = cos $^4$ A

1-cos $^2$ A + 2(1-cos $^2$ A $)^2$ + (1-cos $^2$ A $)^3$ = cos $^4$ A

1-cos$^2$ A + 2-4cos $^2$ A + 2cos $^4$ A + 1- 3cos $^2$ A + 3cos $^4$ A - cos $^6$ A = cos $^4$ A

4 - cos $^6$ A + 4cos $^4$ A - 8cos $^2$ = 0

Therefore cos $^6$ A - 4cos $^4$ A + 8cos $^2$= 0
